new/proof/go_etcd_io/etcd/client/v3/concurrency.v
@@ -56,9 +56,9 @@ Lemma wp_NewSession (client : loc) γetcd :
     func_call #concurrency #"NewSession" #client #slice.nil
   {{{ s err, RET (#s, #err);
       if decide (err = interface.nil) then
-        True
-      else
         is_Session s
+      else
+        True
   }}}.
 Proof.
   wp_start. iNamed "Hpre".
@@ -114,18 +114,61 @@ Proof.
   wp_alloc s as "Hs".
   wp_auto.
   wp_bind (Fork _).
+  iMod (typed_pointsto_persist with "cancel") as "#cancel".
+  iMod (typed_pointsto_persist with "donec") as "#donec".
   iMod (typed_pointsto_persist with "keepAlive") as "#keepAlive".
-  iApply wp_fork.
+  iApply (wp_fork with "[Hdonec Hcancel]").
   {
     iNext.
     wp_auto.
     wp_apply wp_with_defer as "%defer defer".
     simpl subst.
     wp_auto.
-    (* FIXME: spec for chan.for_range *)
-    admit.
+    iDestruct "Hkch" as "#[Hkch #Hkrecv]".
+    wp_for_chan.
+    { iFrame "#". }
+    iAssert _ with "Hkrecv" as "Hkrecv1".
+    iMod "Hkrecv1" as "(% & ? & Hkrecv1)".
+    iFrame. iModIntro. iNext.
+    destruct decide.
+    {
+      iIntros "?".
+      iMod ("Hkrecv1" with "[$]") as "_".
+      iModIntro.
+      wp_auto.
+      iDestruct (own_chan_is_chan with "Hdonec") as "#?".
+      wp_apply (wp_chan_close with "[$] [Hdonec Hcancel]").
+      iApply fupd_mask_intro; [set_solver | iIntros "Hmask"].
+      iNext. iFrame.
+      iSplitR; first done.
+      iIntros "Hdonec".
+      iMod "Hmask".
+      iModIntro.
+      wp_auto.
+      wp_apply "Hcancel".
+      done.
+    }
+    {
+      iIntros "?".
+      iMod ("Hkrecv1" with "[$]") as "_".
+      iModIntro.
+      iMod "Hkrecv" as "(% & $ & Hkrecv)".
+      iModIntro. iNext.
+      iIntros "* _ ?".
+      iMod ("Hkrecv" with "[$]") as "_".
+      iModIntro.
+      wp_auto.
+      wp_for_chan_post.
+      iFrame.
+    }
   }
-
+  iNext.
+  wp_auto.
+  iApply "HΦ".
+  rewrite decide_True //.
+  (* FIXME: avoid putting shelving these things.*)
+  Unshelve.
+  all: try tc_solve.
 Admitted.
 
 End proof.
